Begin separating full typeclasses

Tealeaves/Classes/Full/Monad.v
@@ -4,6 +4,52 @@ From Tealeaves.Classes Require Import
 
 #[local] Generalizable Variables T U A B.
 
+(** * Full Kleisli Typeclasses *)
+(******************************************************************************)
+Class MonadFull (T: Type -> Type)
+  `{Return_T: Return T}
+  `{Map_T: Map T}
+  `{Bind_T: Bind T T} :=
+  { kmonf_kmon:> Monad T;
+    kmonf_map_to_bind:> Compat_Map_Bind T T;
+  }.
+
+Class RightModuleFull (T: Type -> Type) (U: Type -> Type)
+  `{Return_T: Return T}
+  `{Bind_T: Bind T T}
+  `{Bind_TU: Bind T U}
+  `{Map_T: Map T}
+  `{Map_U: Map U}
+  :=
+  { kmodf_mod :> RightModule T U;
+    kmodf_compat :> Compat_Map_Bind T U;
+    kmodf_monad :> MonadFull T;
+  }.
+
+Module FullInstances.
+
+  #[export] Instance MonadFull_Monad
+    (T: Type -> Type)
+    `{Monad_T: Monad T}:
+  MonadFull T
+    (Map_T := Monad.DerivedOperations.Map_Bind T T)
+  :=
+  {| kmonf_map_to_bind := _;
+  |}.
+
+  #[export] Instance RightModuleFull_RightModule
+    (T U: Type -> Type)
+    `{RightModule_TU: RightModule T U}:
+    RightModuleFull T U
+      (Map_T := DerivedOperations.Map_Bind T T)
+      (Map_U := DerivedOperations.Map_Bind T U) :=
+    {| kmodf_monad :=
+        MonadFull_Monad T (Monad_T := kmod_monad)
+    |}.
+
+End FullInstances.
+
+
 (** * Derived Categorical operations *)
 (******************************************************************************)
 Class Compat_Join_Bind
@@ -19,19 +65,23 @@ Class Compat_Join_Bind
       @bind T T bind_T A B f = @join T join_T B ∘ @map T map_T A (T B) f;
   }.
 
+About Compat_Join_Bind.
+
 (** ** Rewriting *)
 (******************************************************************************)
-Lemma join_to_bind:
+Lemma join_to_bind
   `{join_T: Join T}
+  `{return_T: Return T}
+  `{map_T: Map T}
   `{bind_T: Bind T T}
-  `{compat: !Compat_Join_Bind T T}:
-  forall `(f : A -> T B),
-    @join T join_T A = @bind T U bind_U A B (@ret T ret_T B ∘ f).
+  `{compat: !Compat_Join_Bind T}:
+  forall (A: Type),
+    @join T join_T A =
+      @bind T T bind_T (T A) A id.
 Proof.
-  rewrite compat_map_bind.
+  intros. rewrite compat_join_bind.
   reflexivity.
 Qed.
-
 
 Class Monad (T : Type -> Type)
   `{Return_inst: Return T}
@@ -43,15 +93,3 @@ Class Monad (T : Type -> Type)
     fmon_kleisli :> Kleisli.Monad.Monad T;
     fmon_compat :> Compat_Join_Bind T;
   }.
-
-From Tealeaves Require Import
-  Adapters.KleisliToCategorical.Monad.
-
-Import KleisliToCategorical.Monad.Instance.
-
-Print Instances Map.
-
-#[export] Instance MonadFull_Kleisli {T} `{Kleisli.Monad.Monad T}:
-  Full.Monad.Monad T :=
-  {| fmon_cat := CategoricalFromKleisli_Monad T;
-  |}.
