Tealeaves/Classes/Kleisli/Theory/Comonad.v
@@ -1,6 +1,0 @@
-From Tealeaves Require Export
-  Classes.Kleisli.Comonad.
-
-Import Comonad.Notations.
-
-#[local] Generalizable Variables W A B C D.
